src/Std/Tactic/BVDecide/Bitblast/BVExpr/Circuit/Lemmas/Operations/PopCount.lean
@@ -35,87 +35,84 @@ namespace BVExpr
 namespace bitblast
 namespace blastPopCount
 
-/-- Casting `RefVecVec` -/
-def RefVecVec.cast_eq {aig1 aig2 : AIG α} (s : RefVecVec aig1 lenWords len) (h : aig1.decls.size ≤ aig2.decls.size) :
+/-- Casting `RefVecVec` twice is the same as casting once. -/
+theorem RefVecVec.cast_cast {aig1 aig2 : AIG α} (s : RefVecVec aig1 lenWords len) (h : aig1.decls.size ≤ aig2.decls.size) :
     (s.cast h).cast (aig2 := aig2) (by omega) = s.cast h := by
   simp [RefVecVec.cast]
 
-theorem denote_push {aigOld aigNew : AIG α} {n w : Nat}
+/-- Getting the `idx`-th element of the `vec` of `RefVecVec` after setting it retrieves the same element. -/
+theorem RefVecVec.get_set_eq {aigOld aigNew : AIG α} {w len : Nat} (idx : Nat) (s : RefVecVec aigOld w len) (elem : RefVec aigNew w)
+      (h : idx < len) (h' : aigOld.decls.size ≤ aigNew.decls.size) :
+    (RefVecVec.set idx s elem h' h).vec[idx] = elem := by
+  simp [RefVecVec.set]
+
+/-- After setting the `idx`-th element of the `vec` of `RefVecVec`, retrieving any element that is not at that index
+    is the same as getting that element from the original vector. -/
+theorem RefVecVec.get_set {aigOld aigNew : AIG α} {w len : Nat} (idx : Nat) (s : RefVecVec aigOld w len) (elem : RefVec aigNew w)
+      (h : idx < len) (h' : aigOld.decls.size ≤ aigNew.decls.size) :
+  ∀ (idx' : Nat) (_ : ¬idx' = idx) (hi' : idx' < len),
+    (RefVecVec.set idx s elem h' h).vec[idx'] = (s.cast h').vec[idx'] := by
+  intros idx1 hidx1 hidx1'
+  simp only [RefVecVec.set, Vector.getElem_set, Vector.getElem_map, RefVecVec.cast, ite_eq_right_iff]
+  intros
+  omega
+
+theorem denote_set {aigOld aigNew : AIG α} {n w : Nat}
   (acc : RefVecVec aigOld w n) (elem : AIG.RefVec aigNew w)
+  (idxSet : Nat) (hidxSet : idxSet < n)
   (haig : aigOld.decls.size ≤ aigNew.decls.size)
   (assign : α → Bool) (l : List (BitVec w)) (bv : BitVec w)
   (hlen : l.length = n)
   (hvec : ∀ (idx1 : Nat) (hidx1 : idx1 < n),
     ∀ (idx2 : Nat) (hidx2 : idx2 < w),
-      ⟦aigNew, ((acc.cast haig).vec.get ⟨idx1, hidx1⟩).get idx2 hidx2, assign⟧ =
-      (l.get ⟨idx1, by omega⟩).getLsbD idx2)
+      ⟦aigNew, ((acc.cast haig).vec[idx1]).get idx2 hidx2, assign⟧ =
+      l[idx1].getLsbD idx2)
   (helem : ∀ (idx1 : Nat) (hidx1 : idx1 < w),
     ⟦aigNew, elem.get idx1 hidx1, assign⟧ = (bv.getLsbD idx1))
-  : ∀ (idx1 : Nat) (hidx1 : idx1 < n + 1),
-    ∀ (idx2 : Nat) (hidx2 : idx2 < w),
-      ⟦aigNew, ((acc.push elem haig).vec.get ⟨idx1, hidx1⟩).get idx2 hidx2, assign⟧ =
-      ((l.concat bv).get ⟨idx1, by have := List.length_concat (as := l) (a := bv); omega⟩).getLsbD idx2 := by
-  intros idx1 hidx1 idx2 hidx2
-  by_cases hidxlt : idx1 < n
-  · have : (acc.push elem haig).vec.get ⟨idx1, (by omega)⟩ =
-      ((acc.cast haig).vec.get ⟨idx1, (by omega)⟩) := by
-      unfold RefVecVec.push
-      exact Vector.getElem_push_lt (x := elem) (i := idx1) (xs := (Vector.map (fun refVec => refVec.cast haig) acc.vec)) hidxlt
-    simp only [this]
-    have : (l.concat bv).get ⟨idx1, by simp [hlen]; omega⟩ = l.get ⟨idx1, by simp [hlen]; omega⟩ := by
-      have hlen' := List.length_concat (as := l) (a := bv)
-      have := List.getElem_append_left (as := l) (i := idx1) (bs := [bv]) (by simp [hlen]; omega) (h' := by simp; omega)
-      simp [this]
-    rw [this]
-    simp [hvec]
-  · have : idx1 = n := by omega
-    simp only  [this] at *
-    have : (acc.push elem haig).vec.get ⟨n, (by omega)⟩ = elem := by
-      unfold RefVecVec.push
-      exact Vector.getElem_push_last (x := elem) (n := n)
-        (xs := (Vector.map (fun refVec => refVec.cast haig) acc.vec))
-    simp only [this]
-    have : (l.concat bv).get ⟨n, by simp [hlen]⟩ = bv := by
-      have h2 := List.getElem_concat_length (l := l) (i := n) (a := bv) (by simp [hlen])
-      specialize h2 (by simp [hlen])
-      simp [h2]
-    rw [this]
-    simp [helem]
-
-theorem denote_cast {aigCurr aigNew : AIG α} {n w : Nat}
-  (acc : RefVecVec aigCurr w n)
-  (haig : aigCurr.decls.size ≤ aigNew.decls.size)
-  (assign : α → Bool) (l : List (BitVec w))
-  (hlen : l.length = n)
-  (hvec : ∀ (idx1 : Nat) (hidx1 : idx1 < n),
-    ∀ (idx2 : Nat) (hidx2 : idx2 < w),
-      ⟦aigCurr, (acc.vec.get ⟨idx1, hidx1⟩).get idx2 hidx2, assign⟧ = (l.get ⟨idx1, (by omega)⟩).getLsbD idx2)
   : ∀ (idx1 : Nat) (hidx1 : idx1 < n),
     ∀ (idx2 : Nat) (hidx2 : idx2 < w),
-      ⟦aigNew, (((acc.cast haig)).vec.get ⟨idx1, hidx1⟩).get idx2 hidx2, assign⟧ = l[idx1].getLsbD idx2 := by
-  simp [RefVecVec.cast]
-  simp at hvec
+      ⟦aigNew, ((acc.set idxSet elem haig (hidxSet)).vec[idx1]).get idx2 hidx2, assign⟧ =
+      ((l.set idxSet bv)[idx1]'(by simp; omega)).getLsbD idx2 := by
   intros idx1 hidx1 idx2 hidx2
-  rw [← hvec _ (by omega) _ (by omega)]
+  by_cases heq : idxSet = idx1
+  · simp [←heq, RefVecVec.get_set_eq idxSet acc elem hidxSet haig, helem]
+  · simp only [ne_eq, heq, not_false_eq_true, List.getElem_set_ne]
+    rw [RefVecVec.get_set idxSet acc elem hidxSet haig]
+    · apply hvec
+    · omega
 
-  sorry
+-- theorem denote_cast {aigCurr aigNew : AIG α} {n w : Nat}
+--   (acc : RefVecVec aigCurr w n)
+--   (haig : aigCurr.decls.size ≤ aigNew.decls.size)
+--   (assign : α → Bool) (l : List (BitVec w))
+--   (hlen : l.length = n)
+--   (hvec : ∀ (idx1 : Nat) (hidx1 : idx1 < n),
+--     ∀ (idx2 : Nat) (hidx2 : idx2 < w),
+--       ⟦aigCurr, (acc.vec.get ⟨idx1, hidx1⟩).get idx2 hidx2, assign⟧ = (l.get ⟨idx1, (by omega)⟩).getLsbD idx2)
+--   : ∀ (idx1 : Nat) (hidx1 : idx1 < n),
+--     ∀ (idx2 : Nat) (hidx2 : idx2 < w),
+--       ⟦aigNew, (((acc.cast haig)).vec.get ⟨idx1, hidx1⟩).get idx2 hidx2, assign⟧ = l[idx1].getLsbD idx2 := by
+--   simp at hvec
+--   intros idx1 hidx1 idx2 hidx2
+--   specialize hvec idx1 hidx1 idx2 hidx2
+--   sorry
 
-theorem denote_cast_cast {aigCurr aigNew : AIG α} {n w : Nat}
-  (acc : RefVecVec aigCurr w n)
-  (haig : aigCurr.decls.size ≤ aigNew.decls.size)
-  (haig' : aigNew.decls.size ≤ aigNew.decls.size)
-  (assign : α → Bool) (l : List (BitVec w))
-  (hlen : l.length = n)
-  (hvec : ∀ (idx1 : Nat) (hidx1 : idx1 < n),
-    ∀ (idx2 : Nat) (hidx2 : idx2 < w),
-      ⟦aigCurr, (acc.vec.get ⟨idx1, hidx1⟩).get idx2 hidx2, assign⟧ = (l.get ⟨idx1, (by omega)⟩).getLsbD idx2)
-  : ∀ (idx1 : Nat) (hidx1 : idx1 < n),
-    ∀ (idx2 : Nat) (hidx2 : idx2 < w),
-      ⟦aigNew, (((acc.cast haig).cast haig').vec.get ⟨idx1, hidx1⟩).get idx2 hidx2, assign⟧ = l[idx1].getLsbD idx2 := by
-  rw [RefVecVec.cast_eq]
-  intros idx1 hidx1 idx2 hidx2
-  rw [denote_cast (aigNew:=aigNew) (aigCurr:=aigCurr) (haig := haig) (hlen := by omega)]
-  apply hvec
+-- theorem denote_cast_cast {aigCurr aigNew : AIG α} {n w : Nat}
+--   (acc : RefVecVec aigCurr w n)
+--   (haig : aigCurr.decls.size ≤ aigNew.decls.size)
+--   (haig' : aigNew.decls.size ≤ aigNew.decls.size)
+--   (assign : α → Bool) (l : List (BitVec w))
+--   (hlen : l.length = n)
+--   (hvec : ∀ (idx1 : Nat) (hidx1 : idx1 < n),
+--     ∀ (idx2 : Nat) (hidx2 : idx2 < w),
+--       ⟦aigCurr, (acc.vec.get ⟨idx1, hidx1⟩).get idx2 hidx2, assign⟧ = (l.get ⟨idx1, (by omega)⟩).getLsbD idx2)
+--   : ∀ (idx1 : Nat) (hidx1 : idx1 < n),
+--     ∀ (idx2 : Nat) (hidx2 : idx2 < w),
+--       ⟦aigNew, (((acc.cast haig).cast haig').vec.get ⟨idx1, hidx1⟩).get idx2 hidx2, assign⟧ = l[idx1].getLsbD idx2 := by
+--   rw [RefVecVec.cast_eq]
+--   intros idx1 hidx1 idx2 hidx2
+--   rw [denote_cast (aigNew:=aigNew) (aigCurr:=aigCurr) (haig := haig) (hlen := by omega)]
+--   apply hvec
 
 theorem denote_blastExtractAndExtend (aig : AIG α) (xc : AIG.RefVec aig w) (x : BitVec w) (start : Nat)
     (hx : ∀ (idx : Nat) (hidx : idx < w), ⟦aig, xc.get idx hidx, assign⟧ = x.getLsbD idx) :
@@ -128,14 +125,14 @@ theorem denote_blastExtractAndExtend (aig : AIG α) (xc : AIG.RefVec aig w) (x :
   intros idx hidx
   generalize hext: blastExtractAndExtend aig xc start = res
   unfold blastExtractAndExtend at hext
-  dsimp at hext
+  dsimp only [Lean.Elab.WF.paramLet] at hext
   rw [← hext]
-  simp [denote_blastZeroExtend]
+  simp only [denote_blastZeroExtend, Nat.lt_one_iff, denote_blastExtract, dite_eq_ite,
+    Bool.if_false_right, BitVec.truncate_eq_setWidth, BitVec.getLsbD_setWidth,
+    BitVec.getLsbD_extract, Nat.sub_self, Nat.le_zero_eq]
   split
   · by_cases hidx0 : idx = 0
-    · simp [hidx0]
-      simp [show 0 < w by omega]
-      apply hx
+    · simp [hidx0, show 0 < w by omega, hx]
     · simp [hidx0]
   · intros
     simp [show w ≤ start + idx by omega]
@@ -147,210 +144,284 @@ theorem BitVec.extractAndExtendPopulateAux_get
   let out :=  (BitVec.extractAndExtendPopulateAux 0 x [] (by intros i h h'; simp at h') (by omega) (by simp))
   have := (out.property).right
   specialize this i hi (by omega)
-  simp only
-  simp [out] at this
-  simp [this]
+  simp only [List.get_eq_getElem, BitVec.truncate_eq_setWidth, out] at this
+  apply this
 
-theorem denote_eq_blastExtractAndExtendPopulate
-  (assign : α → Bool)
-  (aigAcc : AIG α) (start w : Nat) (xc : AIG.RefVec aigAcc w) (x : BitVec w) (acc : RefVecVec aigAcc w start) (hw : start + 1 < w)
-  (hacc' : ∀ (idx1 : Nat) (hidx1 : idx1 < start),
-            ∀ (idx2 : Nat) (hidx2 : idx2 < w),
-              let newElem := blastExtractAndExtend aigAcc xc (start)
-              ⟦newElem.aig, ((acc.cast (by apply extractAndExtend_le_size)).vec.get ⟨idx1, hidx1⟩).get idx2 hidx2, assign⟧ =
-              ((BitVec.extractAndExtendPopulateAux 0 x [] (by simp) (by omega) (by simp)).val.get
-                ⟨idx1, by simp [(BitVec.extractAndExtendPopulateAux 0 x []
-                        (by intros i hi hl; simp at hl)
-                        (by omega) (by simp)).property]; exact Nat.lt_trans hidx1 (by omega)⟩).getLsbD idx2)
-  (hx : ∀ (idx : Nat) (hidx : idx < w), ⟦aigAcc, xc.get idx hidx, assign⟧ = x.getLsbD idx)
-   :
-    ∀ (idx1 : Nat) (hidx1 : idx1 < start + 1),
-      ∀ (idx2 : Nat) (hidx2 : idx2 < w),
-      ⟦
-        (blastExtractAndExtend aigAcc xc start).aig,
-        (((acc.cast (aig2 := (blastExtractAndExtend aigAcc xc (start)).aig)
-          (by apply extractAndExtend_le_size)).push (blastExtractAndExtend aigAcc xc (start)).vec (by omega)).vec.get ⟨idx1, by omega⟩).get idx2 hidx2,
-        assign
-      ⟧ =
-        let bvRes := BitVec.extractAndExtendPopulateAux 0 x [] (by intros i hi hl; simp at hl) (by omega) (by simp)
-      (bvRes.val.get ⟨idx1, by simp [bvRes.property]; omega⟩).getLsbD idx2 := by
-  -- Introduce a variable `ext` for `blastExtractAndExtend`
-  intros idx1 hidx1 idx2 hidx2
-  let elem := blastExtractAndExtend aigAcc xc start
-  let bvRes := BitVec.extractAndExtendPopulateAux 0 x [] (by intros i hi hl; simp at hl) (by omega) (by simp)
-  let currList := bvRes.val.extract (start := 0) (stop := start)
-  let currElem := bvRes.val.get ⟨start, by omega⟩
-  rw [denote_push (l := currList) (bv := currElem)]
-  · simp
-    by_cases h1 : idx1 = start
-    · -- inspecting the last element of the list
-      simp [h1]
-      have h2 := List.getElem_concat_length (i := start) (a := currElem) (l := currList) (by simp [currList]; omega)
-      specialize h2 (by simp [currList]; omega)
-      simp [h2]
-      let res' := BitVec.extractAndExtendPopulateAux 0 x [] (by intros i hi hl; simp at hl) (by omega) (by simp)
-      have := BitVec.extractAndExtendPopulateAux_get (i := start) (x := x)
-        (hi := by omega) (by omega)
-      simp at this
-      rw [this]
-      simp only [currElem]
-      simp
-      rw [BitVec.extractAndExtendPopulateAux_get (i := start) (x := x) (by have := bvRes; omega) (by omega)]
-      simp
-    · -- inspecting an element that was already in the acc
-      have hl := List.getElem_append_left (as := currList) (bs := [currElem]) (i := idx1) (h' := by simp; omega)
-      rw [hl (by simp [currList];  omega)]
-      let res := BitVec.extractAndExtendPopulateAux 0 x [] (by intros i hi hl; simp at hl) (by omega) (by simp)
-      rw [BitVec.extractAndExtendPopulateAux_get (i := idx1) (x := x) (by have := res; omega) (by omega)]
-      have : idx1 < start := by omega
-      simp [currList]
-      simp [bvRes]
-      rw [BitVec.extractAndExtendPopulateAux_get (i := idx1) (x := x) (by have := bvRes; omega) (by omega)]
-      simp
-  · simp [currList]; omega
-  · intros idx1 hidx1 idx2 hidx2
-    simp [currList, bvRes]
-    simp at hacc'
-    specialize hacc' idx1 hidx1 idx2 hidx2
-    have hproof1 : aigAcc.decls.size ≤ (blastExtractAndExtend aigAcc xc start).aig.decls.size := by apply extractAndExtend_le_size
-    have hproof2 : (blastExtractAndExtend aigAcc xc start).aig.decls.size ≤ (blastExtractAndExtend aigAcc xc start).aig.decls.size := by omega
-    have hcast' : ((acc.cast hproof1).cast hproof2) = acc.cast (by apply extractAndExtend_le_size) := by simp [RefVecVec.cast]
-    rw [hcast']
-    apply hacc'
-  · intros idx hidx
-    rw [denote_blastExtractAndExtend (aig := aigAcc) (xc := xc) (x := x) (start := start) (assign := assign) (hx := hx)]
-    ·
-      simp
-      by_cases h1 : idx = 0
-      · -- this is the only bit that gets actually populated with a meaningful value
-        simp [h1, show 0 < w by omega]
-        simp [currElem]
-        simp [bvRes]
-        have :=  BitVec.extractAndExtendPopulateAux_get (i := start) (x := x) (by omega) (by omega)
-        simp [this]
-      · -- everythign else is the result of zExt
-        simp [h1]
-        simp [currElem, bvRes]
-        have :=  BitVec.extractAndExtendPopulateAux_get (i := start) (x := x) (by omega) (by omega)
-        simp [this]
-        intros
-        omega
+-- theorem denote_eq_blastExtractAndExtendPopulate
+--   (assign : α → Bool)
+--   (aig : AIG α) (start w : Nat) (xc : AIG.RefVec aig w) (x : BitVec w) (acc : RefVecVec aig w w) (hstart : start < w)
+--   -- the bits added already denote to the corresponding entry in acc
+--   (hacc : ∀ (idx1 : Nat) (hidx1 : idx1 < start),
+--             ∀ (idx2 : Nat) (hidx2 : idx2 < w),
+--               let newElem := blastExtractAndExtend aig xc start
+--               ⟦newElem.aig, ((acc.cast (by apply extractAndExtend_le_size)).vec[idx1]).get idx2 hidx2, assign⟧ =
+--               ((BitVec.extractAndExtendPopulateAux 0 x [] (by simp) (by omega) (by simp)).val.get
+--                 ⟨idx1, by simp [(BitVec.extractAndExtendPopulateAux 0 x []
+--                         (by intros i hi hl; simp at hl)
+--                         (by omega) (by simp)).property]; exact Nat.lt_trans hidx1 (by omega)⟩).getLsbD idx2)
+--   -- the remaining entries denote to 0
+--   (hacc' : ∀ (idx1 : Nat) (hidx1 : start ≤ idx1) (hidx1' : idx1 < w),
+--             ∀ (idx2 : Nat) (hidx2 : idx2 < w),
+--               let newElem := blastExtractAndExtend aig xc start
+--               ⟦newElem.aig, ((acc.cast (by apply extractAndExtend_le_size)).vec[idx1]).get idx2 hidx2, assign⟧ = (0#w).getLsbD idx2)
+--   (hx : ∀ (idx : Nat) (hidx : idx < w), ⟦aig, xc.get idx hidx, assign⟧ = x.getLsbD idx)
+--    :
+--     ∀ (idx1 : Nat) (hidx1 : idx1 < start + 1),
+--       ∀ (idx2 : Nat) (hidx2 : idx2 < w),
+--       let bit := blastExtractAndExtend aig xc (start)
+--       let updated := acc.set start bit.vec (by apply extractAndExtend_le_size) hstart
+--       ⟦
+--         bit.aig,
+--         (updated.vec[idx1]).get idx2 hidx2,
+--         assign
+--       ⟧ =
+--         let bvRes := BitVec.extractAndExtendPopulateAux 0 x [] (by intros i hi hl; simp at hl) (by omega) (by simp)
+--       (bvRes.val.get ⟨idx1, by simp [bvRes.property]; omega⟩).getLsbD idx2 := by
+--   intros idx1 hidx1 idx2 hidx2
+--   let bit := blastExtractAndExtend aig xc (start)
+--   let updated := acc.set start bit.vec (by apply extractAndExtend_le_size) hstart
+--   let bvRes := BitVec.extractAndExtendPopulateAux 0 x [] (by intros i hi hl; simp at hl) (by omega) (by simp)
+--   let currList := bvRes.val.extract (start := 0) (stop := start)
+--   let currElem := bvRes.val.get ⟨start, by omega⟩
+--   simp only [List.get_eq_getElem, BitVec.truncate_eq_setWidth]
+--   rw [denote_set (aigOld := aig) (aigNew := bit.aig) (acc := acc) (idxSet := start)
+--           (hidxSet := hstart) (haig := by apply extractAndExtend_le_size) (assign := assign)
+--           (l := bvRes) (hlen := by simp; omega) (bv := currElem)]
+--   · simp [bvRes, currElem, bvRes]
+--   · simp [bit]
+--     intros jdx1 hjdx1 jdx2 hjdx2
+--     by_cases hjdx1' : jdx1 < start
+--     · specialize hacc jdx1 hjdx1' jdx2 hjdx2
+--       apply hacc
+--     · specialize hacc' jdx1 (by omega) (by omega) jdx2 hjdx2
+--       simp at hacc'
+--       by_cases hjdx1' : jdx1 = start
+--       · simp [hjdx1']
+--         have ⟨hlen, hprop⟩ := bvRes.property
+--         specialize hprop start (by omega) (by omega)
+--         simp at hprop
+--         simp [hprop]
 
-theorem BitVec.addVecAux_prop
 
-  (oldParSumBv : List (BitVec w)) (newParSumBv : List (BitVec w))
-  (hlen : oldParSumBv.length = inputNodes)
-  (hlen' : newParSumBv.length = currNode/2)
-  (hle : currNode ≤ inputNodes)
-  (heven : currNode %2 = 0)
-  (hlt : i * 2 + 1 < oldParSumBv.length)
-  (hlt' : i < newParSumBv.length)
-  (res : {l : List (BitVec w) // (l.length = (inputNodes + 1)/2) ∧
-       (∀ i (hi : i < l.length) (hl : l.length = (inputNodes + 1)/2),
-        if hc : i*2 + 1 < oldParSumBv.length then
-          l.get ⟨i, by simp [hl]; omega⟩ = oldParSumBv.get ⟨i*2, by omega⟩ + oldParSumBv.get ⟨i*2 + 1, by omega⟩
-        else
-          l.get ⟨i, by simp [hl]; omega⟩ = oldParSumBv.get ⟨i*2, by omega⟩)
-        })
-  (hacc : ∀ (i_1 : Nat) (hi : i_1 < newParSumBv.length) (_ : newParSumBv.length = currNode / 2),
-            if hc : i_1 * 2 + 1 < oldParSumBv.length then
-              newParSumBv.get ⟨i_1, (by omega)⟩ = oldParSumBv.get ⟨i_1 * 2, (by omega)⟩ + oldParSumBv.get ⟨i_1 * 2 + 1, hc⟩
-                else newParSumBv.get ⟨i_1, (by omega)⟩ = oldParSumBv.get ⟨i_1 * 2, (by omega)⟩) :
-    newParSumBv[i]'hlt' = (oldParSumBv[i * 2]'(by omega) + oldParSumBv[i * 2 + 1]'hlt):= by
-  have ⟨plen, pp⟩ := res.property
-  specialize pp i (by omega) (by omega)
-  simp [hlt] at pp
-  specialize hacc i (by omega) (by omega)
-  simp [hlt] at hacc
-  apply hacc
 
-theorem denote_step_blastAddVec
-  -- blastAddVec input
-  (aigOld : AIG α) (currNode w: Nat) (hi : 1 < inputNodes) (hle : currNode < inputNodes)
-  (assign : α → Bool)
-  (oldParSum : RefVecVec aigOld w inputNodes) (newParSum : RefVecVec aigOld w (currNode/2))
-  (heven : currNode %2 = 0)  (hw : inputNodes ≤ w) (hw' : 1 < inputNodes)
-  (elem : RefVecEntry α w)
-  (helem' :
-    if hc : currNode + 1 < inputNodes then
-      elem = blastAdd aigOld (w := w) ⟨oldParSum.vec.get ⟨currNode, (by omega)⟩, oldParSum.vec.get ⟨currNode + 1, (by omega)⟩⟩
-    else
-      let zero := blastConst aigOld (w := w) 0
-      elem = blastAdd aigOld (w := w) ⟨oldParSum.vec.get ⟨currNode, (by omega)⟩, zero⟩)
-  -- BitVec input
-  (oldParSumBv : List (BitVec w)) (newParSumBv : List (BitVec w)) (elemBv : BitVec w)
-  (hlenOld : oldParSumBv.length = inputNodes) (hlenNew : newParSumBv.length = currNode/2)
-  (hacc : ∀ (i_1 : Nat) (hi : i_1 < newParSumBv.length),
-    newParSumBv.length = currNode / 2 →
-      if hc : i_1 * 2 + 1 < oldParSumBv.length then
-        newParSumBv.get ⟨i_1, hi⟩ = oldParSumBv.get ⟨i_1 * 2, (by omega)⟩ + oldParSumBv.get ⟨i_1 * 2 + 1, hc⟩
-      else newParSumBv.get ⟨i_1, hi⟩ = oldParSumBv.get ⟨i_1 * 2, (by omega)⟩)
-  -- newParSum denotes to newParSumBv
-  (hnew :
-    ∀ (idx1 : Nat) (hidx1 : idx1 < currNode/2),
-      ∀ (idx2 : Nat) (hidx2 : idx2 < w),
-        ⟦elem.aig, ((newParSum.cast (aig2 := elem.aig)
-                    (by split at helem' <;> (simp [helem']; apply AIG.LawfulVecOperator.le_size (f := blastAdd)))
-                    ).vec.get ⟨idx1, hidx1⟩).get idx2 hidx2, assign⟧ =
-          (newParSumBv.get ⟨idx1, by simp [hlenNew]; omega⟩ ).getLsbD idx2)
-  -- elem denotes to elemBv
-  (helem :
-    ∀ (idx1 : Nat) (hidx1 : idx1 < w),
-      ⟦elem.aig, elem.vec.get idx1 hidx1, assign⟧ = elemBv.getLsbD idx1
-    )
-        :
-    ∀ (idx1 : Nat) (hidx1 : idx1 < (currNode + 1)/2),
-      ∀ (idx2 : Nat) (hidx2 : idx2 < w),
-        ⟦elem.aig, ((newParSum.push elem.vec (by split at helem' <;> (simp [helem']; apply AIG.LawfulVecOperator.le_size (f := blastAdd)))).vec.get ⟨idx1, by omega⟩).get idx2 hidx2 , assign⟧ =
-          let bvRes := BitVec.addVecAux 0 inputNodes oldParSumBv [] (by omega) (by omega) (by omega) (by omega) hlenOld (by simp) (by simp)
-          (bvRes.val.get ⟨idx1, by have := bvRes; omega⟩).getLsbD idx2 := by
-    intros idx1 hidx1 idx2 hidx2
-    have := denote_push (assign := assign) (w := w) (n := currNode/2) (aigNew := elem.aig) (aigOld := aigOld)
-          (acc := newParSum) (elem := elem.vec) (l := newParSumBv) (bv := elemBv)
-          (by split at helem' <;> (simp [helem']; apply AIG.LawfulVecOperator.le_size (f := blastAdd))) (by omega)
-    rw [this]
-    · by_cases hlast : idx1 < newParSumBv.length
-      · simp
-        have := List.getElem_append_left (as := newParSumBv) (bs := [elemBv]) (i := idx1) (h := by omega) (h' := by simp; omega)
-        simp [this]
-        let bvRes := BitVec.addVecAux 0 inputNodes oldParSumBv [] (by omega) (by omega) hw hw' hlenOld (by simp) (by omega)
-        have ⟨len, p⟩ := bvRes.property
-        specialize p idx1 (by omega) (by omega)
-        split at p
-        · simp [bvRes] at p
-          simp [p]
-          let bvRes := BitVec.addVecAux 0 inputNodes oldParSumBv [] (by omega) (by omega) hw hw' hlenOld (by simp) (by omega)
-          have hle' : currNode ≤ inputNodes := by omega
-          have := BitVec.addVecAux_prop (i := idx1) (currNode := currNode) (inputNodes := inputNodes) (w := w) (oldParSumBv := oldParSumBv)
-                  (newParSumBv := newParSumBv) (by omega) (by omega)
-                  hle' heven (by omega) (by omega) (res := bvRes) hacc
-          simp [this]
-        · omega
-      · have := List.getElem_concat_length (i := idx1) (a := elemBv) (l := newParSumBv) (by omega)
-        specialize this (by omega)
-        simp
-        rw [this]
-        let bvRes := BitVec.addVecAux 0 inputNodes oldParSumBv [] (by omega) (by omega) hw hw' hlenOld (by omega) (by omega)
-        have := bvRes.property
-        omega
-    · intros idx1 hidx1 idx2 hidx2
-      apply hnew
-    · intros
-      apply helem
+
+--         sorry
+--       ·
+--         sorry
+--   ·
+--     sorry
+
+
+
+
+--   (assign : α → Bool) (l : List (BitVec w)) (bv : BitVec w)
+--   (hlen : l.length = n)
+--   (hvec : ∀ (idx1 : Nat) (hidx1 : idx1 < n),
+--     ∀ (idx2 : Nat) (hidx2 : idx2 < w),
+--       ⟦aigNew, ((acc.cast haig).vec[idx1]).get idx2 hidx2, assign⟧ =
+--       l[idx1].getLsbD idx2)
+--   (helem : ∀ (idx1 : Nat) (hidx1 : idx1 < w),
+--     ⟦aigNew, elem.get idx1 hidx1, assign⟧ = (bv.getLsbD idx1))
+--   : ∀ (idx1 : Nat) (hidx1 : idx1 < n),
+--     ∀ (idx2 : Nat) (hidx2 : idx2 < w),
+--       ⟦aigNew, ((acc.set idxSet elem haig (hidxSet)).vec[idx1]).get idx2 hidx2, assign⟧ =
+--       ((l.set idxSet bv)[idx1]'(by simp; omega)).getLsbD idx2 := by
+--   intros idx1 hidx1 idx2 hidx2
+--   by_cases heq : idxSet = idx1
+--   · simp [←heq, RefVecVec.get_set_eq idxSet acc elem hidxSet haig, helem]
+--   · simp only [ne_eq, heq, not_false_eq_true, List.getElem_set_ne]
+--     rw [RefVecVec.get_set idxSet acc elem hidxSet haig]
+--     · apply hvec
+--     · omega
+
+
+
+
+  -- rw [denote_set]
+
+
+--   intros idx1 hidx1 idx2 hidx2
+--   let elem := blastExtractAndExtend aigAcc xc start
+--   let bvRes := BitVec.extractAndExtendPopulateAux 0 x [] (by intros i hi hl; simp at hl) (by omega) (by simp)
+--   let currList := bvRes.val.extract (start := 0) (stop := start)
+--   let currElem := bvRes.val.get ⟨start, by omega⟩
+--   rw [denote_push (l := currList) (bv := currElem)]
+--   · simp
+--     by_cases h1 : idx1 = start
+--     · -- inspecting the last element of the list
+--       simp [h1]
+--       have h2 := List.getElem_concat_length (i := start) (a := currElem) (l := currList) (by simp [currList]; omega)
+--       specialize h2 (by simp [currList]; omega)
+--       simp [h2]
+--       let res' := BitVec.extractAndExtendPopulateAux 0 x [] (by intros i hi hl; simp at hl) (by omega) (by simp)
+--       have := BitVec.extractAndExtendPopulateAux_get (i := start) (x := x)
+--         (hi := by omega) (by omega)
+--       simp at this
+--       rw [this]
+--       simp only [currElem]
+--       simp
+--       rw [BitVec.extractAndExtendPopulateAux_get (i := start) (x := x) (by have := bvRes; omega) (by omega)]
+--       simp
+--     · -- inspecting an element that was already in the acc
+--       have hl := List.getElem_append_left (as := currList) (bs := [currElem]) (i := idx1) (h' := by simp; omega)
+--       rw [hl (by simp [currList];  omega)]
+--       let res := BitVec.extractAndExtendPopulateAux 0 x [] (by intros i hi hl; simp at hl) (by omega) (by simp)
+--       rw [BitVec.extractAndExtendPopulateAux_get (i := idx1) (x := x) (by have := res; omega) (by omega)]
+--       have : idx1 < start := by omega
+--       simp [currList]
+--       simp [bvRes]
+--       rw [BitVec.extractAndExtendPopulateAux_get (i := idx1) (x := x) (by have := bvRes; omega) (by omega)]
+--       simp
+--   · simp [currList]; omega
+--   · intros idx1 hidx1 idx2 hidx2
+--     simp [currList, bvRes]
+--     simp at hacc'
+--     specialize hacc' idx1 hidx1 idx2 hidx2
+--     have hproof1 : aigAcc.decls.size ≤ (blastExtractAndExtend aigAcc xc start).aig.decls.size := by apply extractAndExtend_le_size
+--     have hproof2 : (blastExtractAndExtend aigAcc xc start).aig.decls.size ≤ (blastExtractAndExtend aigAcc xc start).aig.decls.size := by omega
+--     have hcast' : ((acc.cast hproof1).cast hproof2) = acc.cast (by apply extractAndExtend_le_size) := by simp [RefVecVec.cast]
+--     rw [hcast']
+--     apply hacc'
+--   · intros idx hidx
+--     rw [denote_blastExtractAndExtend (aig := aigAcc) (xc := xc) (x := x) (start := start) (assign := assign) (hx := hx)]
+--     ·
+--       simp
+--       by_cases h1 : idx = 0
+--       · -- this is the only bit that gets actually populated with a meaningful value
+--         simp [h1, show 0 < w by omega]
+--         simp [currElem]
+--         simp [bvRes]
+--         have :=  BitVec.extractAndExtendPopulateAux_get (i := start) (x := x) (by omega) (by omega)
+--         simp [this]
+--       · -- everythign else is the result of zExt
+--         simp [h1]
+--         simp [currElem, bvRes]
+--         have :=  BitVec.extractAndExtendPopulateAux_get (i := start) (x := x) (by omega) (by omega)
+--         simp [this]
+--         intros
+--         omega
+
+-- theorem BitVec.addVecAux_prop
+
+--   (oldParSumBv : List (BitVec w)) (newParSumBv : List (BitVec w))
+--   (hlen : oldParSumBv.length = inputNodes)
+--   (hlen' : newParSumBv.length = currNode/2)
+--   (hle : currNode ≤ inputNodes)
+--   (heven : currNode %2 = 0)
+--   (hlt : i * 2 + 1 < oldParSumBv.length)
+--   (hlt' : i < newParSumBv.length)
+--   (res : {l : List (BitVec w) // (l.length = (inputNodes + 1)/2) ∧
+--        (∀ i (hi : i < l.length) (hl : l.length = (inputNodes + 1)/2),
+--         if hc : i*2 + 1 < oldParSumBv.length then
+--           l.get ⟨i, by simp [hl]; omega⟩ = oldParSumBv.get ⟨i*2, by omega⟩ + oldParSumBv.get ⟨i*2 + 1, by omega⟩
+--         else
+--           l.get ⟨i, by simp [hl]; omega⟩ = oldParSumBv.get ⟨i*2, by omega⟩)
+--         })
+--   (hacc : ∀ (i_1 : Nat) (hi : i_1 < newParSumBv.length) (_ : newParSumBv.length = currNode / 2),
+--             if hc : i_1 * 2 + 1 < oldParSumBv.length then
+--               newParSumBv.get ⟨i_1, (by omega)⟩ = oldParSumBv.get ⟨i_1 * 2, (by omega)⟩ + oldParSumBv.get ⟨i_1 * 2 + 1, hc⟩
+--                 else newParSumBv.get ⟨i_1, (by omega)⟩ = oldParSumBv.get ⟨i_1 * 2, (by omega)⟩) :
+--     newParSumBv[i]'hlt' = (oldParSumBv[i * 2]'(by omega) + oldParSumBv[i * 2 + 1]'hlt):= by
+--   have ⟨plen, pp⟩ := res.property
+--   specialize pp i (by omega) (by omega)
+--   simp [hlt] at pp
+--   specialize hacc i (by omega) (by omega)
+--   simp [hlt] at hacc
+--   apply hacc
+
+-- theorem denote_step_blastAddVec
+--   -- blastAddVec input
+--   (aigOld : AIG α) (currNode w: Nat) (hi : 1 < inputNodes) (hle : currNode < inputNodes)
+--   (assign : α → Bool)
+--   (oldParSum : RefVecVec aigOld w inputNodes) (newParSum : RefVecVec aigOld w (currNode/2))
+--   (heven : currNode %2 = 0)  (hw : inputNodes ≤ w) (hw' : 1 < inputNodes)
+--   (elem : RefVecEntry α w)
+--   (helem' :
+--     if hc : currNode + 1 < inputNodes then
+--       elem = blastAdd aigOld (w := w) ⟨oldParSum.vec.get ⟨currNode, (by omega)⟩, oldParSum.vec.get ⟨currNode + 1, (by omega)⟩⟩
+--     else
+--       let zero := blastConst aigOld (w := w) 0
+--       elem = blastAdd aigOld (w := w) ⟨oldParSum.vec.get ⟨currNode, (by omega)⟩, zero⟩)
+--   -- BitVec input
+--   (oldParSumBv : List (BitVec w)) (newParSumBv : List (BitVec w)) (elemBv : BitVec w)
+--   (hlenOld : oldParSumBv.length = inputNodes) (hlenNew : newParSumBv.length = currNode/2)
+--   (hacc : ∀ (i_1 : Nat) (hi : i_1 < newParSumBv.length),
+--     newParSumBv.length = currNode / 2 →
+--       if hc : i_1 * 2 + 1 < oldParSumBv.length then
+--         newParSumBv.get ⟨i_1, hi⟩ = oldParSumBv.get ⟨i_1 * 2, (by omega)⟩ + oldParSumBv.get ⟨i_1 * 2 + 1, hc⟩
+--       else newParSumBv.get ⟨i_1, hi⟩ = oldParSumBv.get ⟨i_1 * 2, (by omega)⟩)
+--   -- newParSum denotes to newParSumBv
+--   (hnew :
+--     ∀ (idx1 : Nat) (hidx1 : idx1 < currNode/2),
+--       ∀ (idx2 : Nat) (hidx2 : idx2 < w),
+--         ⟦elem.aig, ((newParSum.cast (aig2 := elem.aig)
+--                     (by split at helem' <;> (simp [helem']; apply AIG.LawfulVecOperator.le_size (f := blastAdd)))
+--                     ).vec.get ⟨idx1, hidx1⟩).get idx2 hidx2, assign⟧ =
+--           (newParSumBv.get ⟨idx1, by simp [hlenNew]; omega⟩ ).getLsbD idx2)
+--   -- elem denotes to elemBv
+--   (helem :
+--     ∀ (idx1 : Nat) (hidx1 : idx1 < w),
+--       ⟦elem.aig, elem.vec.get idx1 hidx1, assign⟧ = elemBv.getLsbD idx1
+--     )
+--         :
+--     ∀ (idx1 : Nat) (hidx1 : idx1 < (currNode + 1)/2),
+--       ∀ (idx2 : Nat) (hidx2 : idx2 < w),
+--         ⟦elem.aig, ((newParSum.push elem.vec (by split at helem' <;> (simp [helem']; apply AIG.LawfulVecOperator.le_size (f := blastAdd)))).vec.get ⟨idx1, by omega⟩).get idx2 hidx2 , assign⟧ =
+--           let bvRes := BitVec.addVecAux 0 inputNodes oldParSumBv [] (by omega) (by omega) (by omega) (by omega) hlenOld (by simp) (by simp)
+--           (bvRes.val.get ⟨idx1, by have := bvRes; omega⟩).getLsbD idx2 := by
+--     intros idx1 hidx1 idx2 hidx2
+--     have := denote_push (assign := assign) (w := w) (n := currNode/2) (aigNew := elem.aig) (aigOld := aigOld)
+--           (acc := newParSum) (elem := elem.vec) (l := newParSumBv) (bv := elemBv)
+--           (by split at helem' <;> (simp [helem']; apply AIG.LawfulVecOperator.le_size (f := blastAdd))) (by omega)
+--     rw [this]
+--     · by_cases hlast : idx1 < newParSumBv.length
+--       · simp
+--         have := List.getElem_append_left (as := newParSumBv) (bs := [elemBv]) (i := idx1) (h := by omega) (h' := by simp; omega)
+--         simp [this]
+--         let bvRes := BitVec.addVecAux 0 inputNodes oldParSumBv [] (by omega) (by omega) hw hw' hlenOld (by simp) (by omega)
+--         have ⟨len, p⟩ := bvRes.property
+--         specialize p idx1 (by omega) (by omega)
+--         split at p
+--         · simp [bvRes] at p
+--           simp [p]
+--           let bvRes := BitVec.addVecAux 0 inputNodes oldParSumBv [] (by omega) (by omega) hw hw' hlenOld (by simp) (by omega)
+--           have hle' : currNode ≤ inputNodes := by omega
+--           have := BitVec.addVecAux_prop (i := idx1) (currNode := currNode) (inputNodes := inputNodes) (w := w) (oldParSumBv := oldParSumBv)
+--                   (newParSumBv := newParSumBv) (by omega) (by omega)
+--                   hle' heven (by omega) (by omega) (res := bvRes) hacc
+--           simp [this]
+--         · omega
+--       · have := List.getElem_concat_length (i := idx1) (a := elemBv) (l := newParSumBv) (by omega)
+--         specialize this (by omega)
+--         simp
+--         rw [this]
+--         let bvRes := BitVec.addVecAux 0 inputNodes oldParSumBv [] (by omega) (by omega) hw hw' hlenOld (by omega) (by omega)
+--         have := bvRes.property
+--         omega
+--     · intros idx1 hidx1 idx2 hidx2
+--       apply hnew
+--     · intros
+--       apply helem
 
 theorem denote_blastAddVec
   (assign : α → Bool)
-  (aigCurr : AIG α) (currNode w: Nat) (hi : 1 < inputNodes) (hle : currNode < inputNodes)
-  (oldParSum : RefVecVec aigCurr w inputNodes) (newParSum : RefVecVec aigCurr w newLen)
-  (hleneq: newLen = (currNode/2))
-  (heven : currNode % 2 = 0)  (hw : inputNodes ≤ w) (hw' : 1 < inputNodes)
+  (aigCurr : AIG α) (usedNodes validNodes w: Nat)
+  (oldParSum : RefVecVec aigCurr w inputNodes) (newParSum : RefVecVec aigCurr w inputNodes)
+  (heven : usedNodes % 2 = 0) (hin : 1 < inputNodes) (hval : validNodes ≤ inputNodes)
   -- BitVec input
   (oldParSumBv : List (BitVec w)) (newParSumBv : List (BitVec w))
-  (hlenOld : oldParSumBv.length = inputNodes) (hlenNew : newParSumBv.length = currNode/2)
-  (hacc : ∀ (i_1 : Nat) (hi : i_1 < newParSumBv.length) (hlen : newParSumBv.length = currNode / 2),
-      if hc : i_1 * 2 + 1 < oldParSumBv.length then
-        newParSumBv.get ⟨i_1, hi⟩ = oldParSumBv.get ⟨i_1 * 2, (by omega)⟩ + oldParSumBv.get ⟨i_1 * 2 + 1, hc⟩
-      else newParSumBv.get ⟨i_1, hi⟩ = oldParSumBv.get ⟨i_1 * 2, (by omega)⟩)
+  (hlenOld : oldParSumBv.length = inputNodes) (hlenNew : newParSumBv.length = inputNodes)
+  -- all the bitvectors in newParSumBv in the valid range are the result of summing two bitvecs in the
+  -- old list, while the remaining ones are a copy of the elements in the old bitvec.
+  (hacc : ∀ (j : Nat) (hj : j < newParSumBv.length) (hjo : j * 2 < oldParSumBv.length),
+      if hlt : j < (validNodes + 1)/2 then
+        if hc : j * 2 + 1 < oldParSumBv.length then
+          newParSumBv.get ⟨j, hj⟩ = oldParSumBv.get ⟨j * 2, (by omega)⟩ + oldParSumBv.get ⟨j * 2 + 1, hc⟩
+        else
+          newParSumBv.get ⟨j, hj⟩ = oldParSumBv.get ⟨j * 2, (by omega)⟩
+      else
+        newParSumBv.get ⟨j, hj⟩ = oldParSumBv.get ⟨j, by omega⟩
+  )
   -- newParSum denotes to newParSumBv
   (hnew :
     ∀ (idx1 : Nat) (hidx1 : idx1 < currNode/2),
@@ -524,15 +595,15 @@ theorem denote_blastAddVec
           sorry
     · omega
 
-@[simp]
-theorem denote_blastPopCount (aig : AIG α) (xc : RefVec aig w) (x : BitVec w) (assign : α → Bool)
-      (hx : ∀ (idx : Nat) (hidx : idx < w), ⟦aig, xc.get idx hidx, assign⟧ = x.getLsbD idx)
-      :
-      ∀ (idx : Nat) (hidx : idx < w),
-        ⟦(blastPopCount aig xc).aig, (blastPopCount aig xc).vec.get idx hidx, assign⟧
-          =
-        (BitVec.popCountAuxRec x 0 0).getLsbD idx := by
-  sorry
+-- @[simp]
+-- theorem denote_blastPopCount (aig : AIG α) (xc : RefVec aig w) (x : BitVec w) (assign : α → Bool)
+--       (hx : ∀ (idx : Nat) (hidx : idx < w), ⟦aig, xc.get idx hidx, assign⟧ = x.getLsbD idx)
+--       :
+--       ∀ (idx : Nat) (hidx : idx < w),
+--         ⟦(blastPopCount aig xc).aig, (blastPopCount aig xc).vec.get idx hidx, assign⟧
+--           =
+--         (BitVec.popCountAuxRec x 0 0).getLsbD idx := by
+--   sorry
 
 
 
